lim x->1(2x+1)
x=1
2.1+1=3
lim x->1(3)
-----------------------------------------------------------------------------------------------
Lim x->1 (√x+x)
x=1
√1+1
Lim x->1 (2)
-----------------------------------------------------------------------------------------------
Lim x->0(x²-x/x)
x²-x = x.(x-1)
x.(x-1)/x
Lim x->0(x-1)
Lim x->0(-1)
----------------------------------------------------------------------------------------------
Lim x->1/2(4x²-1/2x-1)
Lim x->1/2(2².x²-1²/2x-1)
Lim x->1/2((2x²)-1²/2x-1)->2x+1 . 2x-1 /2x -1
Lim x->1/2(2x+1)
Lim x->1/2(2)
-----------------------------------------------------------------------------------------------
Lim x->1(x³-1/x²-1)
Lim x->1((x-1).(x²+x+1²)/(x+1).(x-1))
Lim x->1(x²+x+1)/x+1
Lim x->1(1+1+1)/1+1
Lim x->1(3/2)
----------------------------------------------------------------------------------------------------------------------------------------------------------------------------------------------
Lim x->1 f(x) , tq f(x)= {se x!=1, x²-1/x-1}
				    {se x=1, 3          }
f(1)---> Lim x->1 (3)
f(x)---> Lim x->1((x+1).(x-1)/x-1)
		Lim x->1(x+1)
		Lim x->1(2)
-----------------------------------------------------------------------------------------------
1 f(x)= {se x!=0, x²-x/x ou L se x=0}
f(x) = x-1
f(x) = 0-1
f(x) = -1
-----------------------------------------------------------------------------------------------
2